Cleaned up typechecking definitions

02Typed/Typechecking.thy
@@ -2,24 +2,6 @@ theory Typechecking
   imports TypedLanguage UnifiableType
 begin
 
-primrec hsubst :: "subst \<Rightarrow> uterm expr\<^sub>s \<Rightarrow> uterm expr\<^sub>s" where
-  "hsubst sub (Var\<^sub>s x) = Var\<^sub>s x"
-| "hsubst sub (Const\<^sub>s k) = Const\<^sub>s k"
-| "hsubst sub (Lam\<^sub>s x t e) = Lam\<^sub>s x (subst sub t) (hsubst sub e)"
-| "hsubst sub (App\<^sub>s e\<^sub>1 e\<^sub>2) = App\<^sub>s (hsubst sub e\<^sub>1) (hsubst sub e\<^sub>2)"
-
-primrec erase :: "'a expr\<^sub>s \<Rightarrow> unit expr\<^sub>s" where
-  "erase (Var\<^sub>s x) = Var\<^sub>s x"
-| "erase (Const\<^sub>s k) = Const\<^sub>s k"
-| "erase (Lam\<^sub>s x t e) = Lam\<^sub>s x () (erase e)"
-| "erase (App\<^sub>s e\<^sub>1 e\<^sub>2) = App\<^sub>s (erase e\<^sub>1) (erase e\<^sub>2)"
-
-primrec htvars :: "uterm expr\<^sub>s \<Rightarrow> var set" where
-  "htvars (Var\<^sub>s x) = {}"
-| "htvars (Const\<^sub>s k) = {}"
-| "htvars (Lam\<^sub>s x t e) = uvars t \<union> htvars e"
-| "htvars (App\<^sub>s e\<^sub>1 e\<^sub>2) = htvars e\<^sub>1 \<union> htvars e\<^sub>2"
-
 primrec typecheck' :: "subst \<Rightarrow> var set \<Rightarrow> 'a expr\<^sub>s \<Rightarrow> uterm expr\<^sub>s \<times> uterm \<times> var set \<times> constraint" 
     where
   "typecheck' \<Gamma> vs (Var\<^sub>s x) = (case \<Gamma> x of 
@@ -35,37 +17,6 @@ primrec typecheck' :: "subst \<Rightarrow> var set \<Rightarrow> 'a expr\<^sub>s
     in let (e\<^sub>1', t\<^sub>1, vs', con\<^sub>1) = typecheck' \<Gamma> (insert v vs) e\<^sub>1 
     in let (e\<^sub>2', t\<^sub>2, vs'', con\<^sub>2) = typecheck' \<Gamma> vs' e\<^sub>2 
     in (App\<^sub>s e\<^sub>1' e\<^sub>2', Var v, vs'', con\<^sub>1 @ con\<^sub>2 @ [(t\<^sub>1, Arrow\<^sub>\<tau> t\<^sub>2 (Var v))]))"
-
-primrec solidify :: "uterm expr\<^sub>s \<Rightarrow> ty expr\<^sub>s" where
-  "solidify (Var\<^sub>s x) = Var\<^sub>s x"
-| "solidify (Const\<^sub>s k) = Const\<^sub>s k"
-| "solidify (Lam\<^sub>s x t e) = Lam\<^sub>s x (to_type t) (solidify e)"
-| "solidify (App\<^sub>s e\<^sub>1 e\<^sub>2) = App\<^sub>s (solidify e\<^sub>1) (solidify e\<^sub>2)"
-
-primrec liquify :: "ty expr\<^sub>s \<Rightarrow> uterm expr\<^sub>s" where
-  "liquify (Var\<^sub>s x) = Var\<^sub>s x"
-| "liquify (Const\<^sub>s k) = Const\<^sub>s k"
-| "liquify (Lam\<^sub>s x t e) = Lam\<^sub>s x (to_unifiable t) (liquify e)"
-| "liquify (App\<^sub>s e\<^sub>1 e\<^sub>2) = App\<^sub>s (liquify e\<^sub>1) (liquify e\<^sub>2)"
-
-primrec partial_solidify :: "var set \<Rightarrow> uterm expr\<^sub>s \<Rightarrow> uterm expr\<^sub>s" where
-  "partial_solidify vs (Var\<^sub>s x) = Var\<^sub>s x"
-| "partial_solidify vs (Const\<^sub>s k) = Const\<^sub>s k"
-| "partial_solidify vs (Lam\<^sub>s x t e) = Lam\<^sub>s x (eliminate_vars vs t) (partial_solidify vs e)"
-| "partial_solidify vs (App\<^sub>s e\<^sub>1 e\<^sub>2) = App\<^sub>s (partial_solidify vs e\<^sub>1) (partial_solidify vs e\<^sub>2)"
-
-fun typecheck :: "'a expr\<^sub>s \<rightharpoonup> ty expr\<^sub>s \<times> ty" where
-  "typecheck e = (
-    let (e', t, vs, con) = typecheck' Map.empty {} e
-    in case unify con of 
-        Some sub \<Rightarrow> Some (solidify (hsubst sub e'), to_type (subst sub t))
-      | None \<Rightarrow> None)"
-
-primrec valid_ty_hexpr :: "uterm expr\<^sub>s \<Rightarrow> bool" where
-  "valid_ty_hexpr (Var\<^sub>s x) = True"
-| "valid_ty_hexpr (Const\<^sub>s k) = True"
-| "valid_ty_hexpr (Lam\<^sub>s x t e) = (valid_ty_term t \<and> valid_ty_hexpr e)"
-| "valid_ty_hexpr (App\<^sub>s e\<^sub>1 e\<^sub>2) = (valid_ty_hexpr e\<^sub>1 \<and> valid_ty_hexpr e\<^sub>2)"
 
 lemma typecheck_induct [consumes 1, case_names Var\<^sub>sS Var\<^sub>sN Const\<^sub>s Lam\<^sub>s App\<^sub>s]: "
   typecheck' \<Gamma> vs e = (e', t, vs', con) \<Longrightarrow> 
@@ -84,68 +35,91 @@ lemma typecheck_induct [consumes 1, case_names Var\<^sub>sS Var\<^sub>sN Const\<
   by (induction e arbitrary: \<Gamma> vs e' t vs' con) 
      (auto simp add: Let_def split: option.splits prod.splits)
 
-lemma [simp]: "valid_ty_hexpr (liquify e)"
+fun typecheck :: "'a expr\<^sub>s \<rightharpoonup> ty expr\<^sub>s \<times> ty" where
+  "typecheck e = (
+    let (e', t, vs, con) = typecheck' Map.empty {} e
+    in case unify con of 
+        Some sub \<Rightarrow> Some (map_expr\<^sub>s to_type (map_expr\<^sub>s (subst sub) e'), to_type (subst sub t))
+      | None \<Rightarrow> None)"
+
+abbreviation erase :: "'a expr\<^sub>s \<Rightarrow> unit expr\<^sub>s" where
+  "erase \<equiv> map_expr\<^sub>s (\<lambda>x. ())"
+
+primrec tyvars\<^sub>s :: "uterm expr\<^sub>s \<Rightarrow> var set" where
+  "tyvars\<^sub>s (Var\<^sub>s x) = {}"
+| "tyvars\<^sub>s (Const\<^sub>s k) = {}"
+| "tyvars\<^sub>s (Lam\<^sub>s x t e) = uvars t \<union> tyvars\<^sub>s e"
+| "tyvars\<^sub>s (App\<^sub>s e\<^sub>1 e\<^sub>2) = tyvars\<^sub>s e\<^sub>1 \<union> tyvars\<^sub>s e\<^sub>2"
+
+primrec valid_ty_expr :: "uterm expr\<^sub>s \<Rightarrow> bool" where
+  "valid_ty_expr (Var\<^sub>s x) = True"
+| "valid_ty_expr (Const\<^sub>s k) = True"
+| "valid_ty_expr (Lam\<^sub>s x t e) = (valid_ty_term t \<and> valid_ty_expr e)"
+| "valid_ty_expr (App\<^sub>s e\<^sub>1 e\<^sub>2) = (valid_ty_expr e\<^sub>1 \<and> valid_ty_expr e\<^sub>2)"
+
+lemma [simp]: "valid_ty_expr (map_expr\<^sub>s to_unifiable e)"
   by (induction e) simp_all
 
-lemma [simp]: "x \<notin> htvars e \<Longrightarrow> hsubst [x \<mapsto> t] e = e"
+lemma [simp]: "x \<notin> tyvars\<^sub>s e \<Longrightarrow> map_expr\<^sub>s (subst [x \<mapsto> t]) e = e"
   by (induction e) simp_all
 
-lemma [simp]: "hsubst (extend_subst x t s) e = hsubst s (hsubst [x \<mapsto> t] e)"
-  by (induction e) (simp_all only: hsubst.simps expand_extend_subst comp_def)
+lemma [simp]: "map_expr\<^sub>s (subst (extend_subst x t s)) e = 
+    map_expr\<^sub>s (subst s) (map_expr\<^sub>s (subst [x \<mapsto> t]) e)"
+  by (induction e) (simp_all only: expr\<^sub>s.map expand_extend_subst comp_def)
 
-lemma [simp]: "solidify (liquify e) = e"
+lemma [simp]: "map_expr\<^sub>s to_type (map_expr\<^sub>s to_unifiable e) = e"
   by (induction e) simp_all
 
-lemma [simp]: "valid_ty_hexpr e \<Longrightarrow> htvars e = {} \<Longrightarrow> liquify (solidify e) = e"
+lemma [simp]: "valid_ty_expr e \<Longrightarrow> tyvars\<^sub>s e = {} \<Longrightarrow> map_expr\<^sub>s to_unifiable (map_expr\<^sub>s to_type e) = e"
   by (induction e) simp_all
 
-lemma [simp]: "erase (solidify (hsubst sub e)) = erase (solidify e)"
+lemma [simp]: "erase (map_expr\<^sub>s to_type (map_expr\<^sub>s (subst sub) e)) = erase (map_expr\<^sub>s to_type e)"
   by (induction e) simp_all
 
-lemma [simp]: "htvars t = {} \<Longrightarrow> partial_solidify vs t = t"
+lemma [simp]: "tyvars\<^sub>s t = {} \<Longrightarrow> map_expr\<^sub>s (eliminate_vars vs) t = t"
   by (induction t) simp_all
 
-lemma [simp]: "x \<notin> htvars t \<Longrightarrow> partial_solidify (insert x vs) t = partial_solidify vs t"
+lemma [simp]: "x \<notin> tyvars\<^sub>s t \<Longrightarrow> map_expr\<^sub>s (eliminate_vars (insert x vs)) t = map_expr\<^sub>s (eliminate_vars vs) t"
   by (induction t) simp_all
 
-lemma [simp]: "valid_ty_subst sub \<Longrightarrow> valid_ty_hexpr e \<Longrightarrow> valid_ty_hexpr (hsubst sub e)"
+lemma [simp]: "valid_ty_subst sub \<Longrightarrow> valid_ty_expr e \<Longrightarrow> valid_ty_expr (map_expr\<^sub>s (subst sub) e)"
   by (induction e) simp_all
 
-lemma htvars_hsubst [simp]: "htvars (hsubst sub e) \<subseteq> htvars e - dom sub \<union> subst_vars sub"
+lemma htvars_hsubst [simp]: "tyvars\<^sub>s (map_expr\<^sub>s (subst sub) e) \<subseteq> tyvars\<^sub>s e - dom sub \<union> subst_vars sub"
 proof (induction e)
   case (Lam\<^sub>s x t e)
   moreover have "uvars (subst sub t) \<subseteq> uvars t - dom sub \<union> subst_vars sub" by simp
   ultimately show ?case by fastforce
 qed auto
 
-lemma [simp]: "dom sub \<inter> htvars e = {} \<Longrightarrow> hsubst sub e = e"
+lemma [simp]: "dom sub \<inter> tyvars\<^sub>s e = {} \<Longrightarrow> map_expr\<^sub>s (subst sub) e = e"
 proof (induction e)
   case (Lam\<^sub>s x t e)
   moreover hence "dom sub \<inter> uvars t = {}" by auto
   ultimately show ?case by auto
 qed auto
 
-lemma [simp]: "hsubst (combine_subst s t) e = hsubst s (hsubst t e)"
+lemma [simp]: "map_expr\<^sub>s (subst (combine_subst s t)) e = map_expr\<^sub>s (subst s) (map_expr\<^sub>s (subst t) e)"
   by (induction e) simp_all
 
 lemma [elim]: "typecheck' \<Gamma> vs e = (e', t, vs', con) \<Longrightarrow> valid_ty_subst \<Gamma> \<Longrightarrow> valid_ty_term t"
   by (induction rule: typecheck_induct) auto
 
-lemma [elim]: "typecheck' \<Gamma> vs e = (e', t, vs', con) \<Longrightarrow> valid_ty_subst \<Gamma> \<Longrightarrow> valid_ty_hexpr e'"
+lemma [elim]: "typecheck' \<Gamma> vs e = (e', t, vs', con) \<Longrightarrow> valid_ty_subst \<Gamma> \<Longrightarrow> valid_ty_expr e'"
   by (induction rule: typecheck_induct) auto
 
 lemma typecheck_succeeds [simp]: "typecheck' \<Gamma> vs e = (e', t, vs', con) \<Longrightarrow> 
   valid_ty_subst \<Gamma> \<Longrightarrow> unify con = Some sub' \<Longrightarrow> sub specializes sub' \<Longrightarrow>
-    map_option (to_type \<circ> subst sub) \<circ> \<Gamma> \<turnstile>\<^sub>t solidify (hsubst sub e') : to_type (subst sub t)"
+    map_option (to_type \<circ> subst sub) \<circ> \<Gamma> \<turnstile>\<^sub>t map_expr\<^sub>s to_type (map_expr\<^sub>s (subst sub) e') : to_type (subst sub t)"
 proof (induction arbitrary: sub' rule: typecheck_induct)
   case (Var\<^sub>sS \<Gamma> vs t x)
   thus ?case by simp
 next
   case (Lam\<^sub>s \<Gamma> vs vs' con x u e\<^sub>1 e\<^sub>1' t' v)
   hence "valid_ty_subst (\<Gamma>(x \<mapsto> Var v))" by simp
-  with Lam\<^sub>s have "map_option (to_type \<circ> subst sub) \<circ> \<Gamma>(x \<mapsto> Var v) \<turnstile>\<^sub>t solidify (hsubst sub e\<^sub>1') : 
+  with Lam\<^sub>s have "map_option (to_type \<circ> subst sub) \<circ> \<Gamma>(x \<mapsto> Var v) \<turnstile>\<^sub>t map_expr\<^sub>s to_type (map_expr\<^sub>s (subst sub) e\<^sub>1') : 
       to_type (subst sub t')" by blast
-  hence "map_option (to_type \<circ> subst sub) \<circ> \<Gamma> \<turnstile>\<^sub>t solidify (hsubst sub (Lam\<^sub>s x (Var v) e\<^sub>1')) :
+  hence "map_option (to_type \<circ> subst sub) \<circ> \<Gamma> \<turnstile>\<^sub>t map_expr\<^sub>s to_type (map_expr\<^sub>s (subst sub) (Lam\<^sub>s x (Var v) e\<^sub>1')) :
     to_type (subst sub (Arrow\<^sub>\<tau> (Var v) t'))" by simp
   thus ?case by blast
 next
@@ -153,7 +127,7 @@ next
   then obtain s\<^sub>2 where S2: "unify (con\<^sub>1 @ con\<^sub>2) = Some s\<^sub>2 \<and> sub' specializes s\<^sub>2" by fastforce
   then obtain s\<^sub>3 where S3: "unify con\<^sub>1 = Some s\<^sub>3 \<and> s\<^sub>2 specializes s\<^sub>3" by fastforce
   with App\<^sub>s S2 have "sub specializes s\<^sub>3" by auto
-  with App\<^sub>s S2 S3 have T: "map_option (to_type \<circ> subst sub) \<circ> \<Gamma> \<turnstile>\<^sub>t solidify (hsubst sub e\<^sub>1') : 
+  with App\<^sub>s S2 S3 have T: "map_option (to_type \<circ> subst sub) \<circ> \<Gamma> \<turnstile>\<^sub>t map_expr\<^sub>s to_type (map_expr\<^sub>s (subst sub) e\<^sub>1') : 
     to_type (subst sub t\<^sub>1)" by blast
   from App\<^sub>s have "sub' unifies\<^sub>\<kappa> (con\<^sub>1 @ con\<^sub>2 @ [(t\<^sub>1, Arrow\<^sub>\<tau> t\<^sub>2 (Var v))])" 
     by (metis unify_some) 
@@ -162,9 +136,9 @@ next
   from S2 obtain s\<^sub>4 where S4: "unify con\<^sub>2 = Some s\<^sub>4 \<and> s\<^sub>2 specializes s\<^sub>4" 
     using unify_append_snd by blast
   with App\<^sub>s S2 have "sub specializes s\<^sub>4" by auto
-  with App\<^sub>s S4 have "map_option (to_type \<circ> subst sub) \<circ> \<Gamma> \<turnstile>\<^sub>t solidify (hsubst sub e\<^sub>2') : 
+  with App\<^sub>s S4 have "map_option (to_type \<circ> subst sub) \<circ> \<Gamma> \<turnstile>\<^sub>t map_expr\<^sub>s to_type (map_expr\<^sub>s (subst sub) e\<^sub>2') : 
     to_type (subst sub t\<^sub>2)" by blast
-  with T X have "map_option (to_type \<circ> subst sub) \<circ> \<Gamma> \<turnstile>\<^sub>t solidify (hsubst sub (App\<^sub>s e\<^sub>1' e\<^sub>2')) : 
+  with T X have "map_option (to_type \<circ> subst sub) \<circ> \<Gamma> \<turnstile>\<^sub>t map_expr\<^sub>s to_type (map_expr\<^sub>s (subst sub) (App\<^sub>s e\<^sub>1' e\<^sub>2')) : 
     to_type (subst sub (Var v))" by simp
   thus ?case by blast
 qed simp_all
@@ -173,15 +147,15 @@ lemma [simp]: "typecheck e = Some (e\<^sub>t, t) \<Longrightarrow> Map.empty \<t
 proof -
   assume "typecheck e = Some (e\<^sub>t, t)"
   then obtain e' tt vs con sub where T: "typecheck' Map.empty {} e = (e', tt, vs, con) \<and>
-    unify con = Some sub \<and> e\<^sub>t = solidify (hsubst sub e') \<and> t = to_type (subst sub tt)" 
+    unify con = Some sub \<and> e\<^sub>t = map_expr\<^sub>s to_type (map_expr\<^sub>s (subst sub) e') \<and> t = to_type (subst sub tt)" 
       by (auto split: option.splits prod.splits)
-  moreover hence "map_option (to_type \<circ> subst sub) \<circ> Map.empty \<turnstile>\<^sub>t solidify (hsubst sub e') : 
+  moreover hence "map_option (to_type \<circ> subst sub) \<circ> Map.empty \<turnstile>\<^sub>t map_expr\<^sub>s to_type (map_expr\<^sub>s (subst sub) e') : 
     to_type (subst sub tt)" by (metis typecheck_succeeds valid_empty_subst specializes_refl)
-  moreover from T have "valid_ty_term tt" and "valid_ty_hexpr e'" by auto
+  moreover from T have "valid_ty_term tt" and "valid_ty_expr e'" by auto
   ultimately show "Map.empty \<turnstile>\<^sub>t e\<^sub>t : t" by simp
 qed
 
-lemma [simp]: "typecheck' \<Gamma> vs e = (e', t, vs', con) \<Longrightarrow> e = erase (solidify e')"
+lemma [simp]: "typecheck' \<Gamma> vs e = (e', t, vs', con) \<Longrightarrow> e = erase (map_expr\<^sub>s to_type e')"
   by (induction rule: typecheck_induct) auto
 
 lemma [simp]: "typecheck e = Some (e\<^sub>t, t) \<Longrightarrow> e = erase e\<^sub>t"
@@ -204,7 +178,7 @@ lemma [simp]: "typecheck' \<Gamma> vs e = (e', t, vs', con) \<Longrightarrow> fi
   by (induction e arbitrary: \<Gamma> vs e' t vs' con) 
      (simp_all add: Let_def split: option.splits prod.splits)
 
-lemma [simp]: "typecheck' \<Gamma> vs e = (e', t', vs', con) \<Longrightarrow> finite vs \<Longrightarrow> htvars e' \<subseteq> vs' - vs"
+lemma [simp]: "typecheck' \<Gamma> vs e = (e', t', vs', con) \<Longrightarrow> finite vs \<Longrightarrow> tyvars\<^sub>s e' \<subseteq> vs' - vs"
 proof (induction rule: typecheck_induct)
   case (Lam\<^sub>s \<Gamma> vs vs' con x u e\<^sub>1 e\<^sub>1' t' v)
   moreover hence "insert v vs \<subseteq> vs'" by (metis vars_expand)
@@ -216,13 +190,13 @@ next
   ultimately show ?case by auto
 qed simp_all
 
-lemma [simp]: "typecheck' \<Gamma> vs e = (e', t', vs', con) \<Longrightarrow> x \<in> vs \<Longrightarrow> finite vs \<Longrightarrow> x \<notin> htvars e'"
+lemma [simp]: "typecheck' \<Gamma> vs e = (e', t', vs', con) \<Longrightarrow> x \<in> vs \<Longrightarrow> finite vs \<Longrightarrow> x \<notin> tyvars\<^sub>s e'"
 proof -
   assume "typecheck' \<Gamma> vs e = (e', t', vs', con)"
      and "finite vs"
-  hence "htvars e' \<subseteq> vs' - vs" by simp
+  hence "tyvars\<^sub>s e' \<subseteq> vs' - vs" by simp
   moreover assume "x \<in> vs" 
-  ultimately show "x \<notin> htvars e'" by auto
+  ultimately show "x \<notin> tyvars\<^sub>s e'" by auto
 qed
 
 lemma [simp]: "typecheck' \<Gamma> vs e = (e', t', vs', con) \<Longrightarrow> finite vs \<Longrightarrow> 
@@ -282,7 +256,7 @@ qed
 
 lemma [simp]: "typecheck' (\<Gamma>(x \<mapsto> Var y)) vs e = (e', tt, vs', con) \<Longrightarrow> y \<in> vs \<Longrightarrow>
   subst_vars \<Gamma> \<subseteq> vs - {y} \<Longrightarrow> uvars t' \<subseteq> vs - {y} \<Longrightarrow> finite vs \<Longrightarrow> typecheck' (\<Gamma>(x \<mapsto> t')) vs e = 
-    (hsubst [y \<mapsto> t'] e', subst [y \<mapsto> t'] tt, vs', constr_subst y t' con)"
+    (map_expr\<^sub>s (subst [y \<mapsto> t']) e', subst [y \<mapsto> t'] tt, vs', constr_subst y t' con)"
 proof (induction e arbitrary: \<Gamma> vs e' tt vs' con)
   case (Var\<^sub>s z)
   thus ?case
@@ -293,7 +267,7 @@ proof (induction e arbitrary: \<Gamma> vs e' tt vs' con)
       case (Some t)
       from Var\<^sub>s have "y \<notin> subst_vars \<Gamma>" by auto
       with Var\<^sub>s False Some have "typecheck' (\<Gamma>(x \<mapsto> t')) vs (Var\<^sub>s z) =
-        (hsubst [y \<mapsto> t'] e', subst [y \<mapsto> t'] tt, vs', constr_subst y t' con)" 
+        (map_expr\<^sub>s (subst [y \<mapsto> t']) e', subst [y \<mapsto> t'] tt, vs', constr_subst y t' con)" 
           by auto
       thus ?thesis by blast
     qed auto
@@ -314,7 +288,7 @@ next
     from Lam\<^sub>s(4) F have "y \<notin> subst_vars (\<Gamma>(z \<mapsto> Var ?v))" 
       by (auto simp add: subst_vars_def ran_def)
     with Lam\<^sub>s F E T' True T have "typecheck' (\<Gamma>(x \<mapsto> t')) vs (Lam\<^sub>s z u e) =
-      (hsubst [y \<mapsto> t'] e', subst [y \<mapsto> t'] tt, vs', constr_subst y t' con)" 
+      (map_expr\<^sub>s (subst [y \<mapsto> t']) e', subst [y \<mapsto> t'] tt, vs', constr_subst y t' con)" 
         by (simp add: Let_def split: if_splits prod.splits)
     thus ?thesis by blast
   next
@@ -327,12 +301,12 @@ next
     have "subst_vars (\<Gamma>(z := None)) \<subseteq> subst_vars \<Gamma>" by simp
     with Lam\<^sub>s(4) F have "subst_vars (\<Gamma>(z \<mapsto> Var ?v)) \<subseteq> insert ?v vs - {y}" by fastforce
     with Lam\<^sub>s X have "typecheck' (\<Gamma>(z \<mapsto> Var ?v, x \<mapsto> t')) (insert ?v vs) e = 
-      (hsubst [y \<mapsto> t'] e'', subst [y \<mapsto> t'] tt', vs', constr_subst y t' con)" by blast
+      (map_expr\<^sub>s (subst [y \<mapsto> t']) e'', subst [y \<mapsto> t'] tt', vs', constr_subst y t' con)" by blast
     with False have "typecheck' (\<Gamma>(x \<mapsto> t', z \<mapsto> Var ?v)) (insert ?v vs) e = 
-      (hsubst [y \<mapsto> t'] e'', subst [y \<mapsto> t'] tt', vs', constr_subst y t' con)" 
+      (map_expr\<^sub>s (subst [y \<mapsto> t']) e'', subst [y \<mapsto> t'] tt', vs', constr_subst y t' con)" 
         by (metis fun_upd_twist)
     with E F have "typecheck' (\<Gamma>(x \<mapsto> t')) vs (Lam\<^sub>s z u e) =
-      (hsubst [y \<mapsto> t'] e', subst [y \<mapsto> t'] tt, vs', constr_subst y t' con)" 
+      (map_expr\<^sub>s (subst [y \<mapsto> t']) e', subst [y \<mapsto> t'] tt, vs', constr_subst y t' con)" 
         by (simp add: Let_def split: if_splits prod.splits)
     thus ?thesis by blast
   qed
@@ -352,17 +326,17 @@ next
   from App\<^sub>s V have C: "uvars t' \<subseteq> vs'' - {y}" by auto
   from App\<^sub>s T1 have D: "finite vs''" by simp
   from App\<^sub>s T1 have T1': "typecheck' (\<Gamma>(x \<mapsto> t')) (insert ?v vs) e1 = 
-    (hsubst [y \<mapsto> t'] e\<^sub>1', subst [y \<mapsto> t'] t\<^sub>1, vs'', constr_subst y t' con\<^sub>1)" by blast
+    (map_expr\<^sub>s (subst [y \<mapsto> t']) e\<^sub>1', subst [y \<mapsto> t'] t\<^sub>1, vs'', constr_subst y t' con\<^sub>1)" by blast
   from App\<^sub>s T2 A B C D have T2': "typecheck' (\<Gamma>(x \<mapsto> t')) vs'' e2 = 
-    (hsubst [y \<mapsto> t'] e\<^sub>2', subst [y \<mapsto> t'] t\<^sub>2, vs''', constr_subst y t' con\<^sub>2)" by blast
+    (map_expr\<^sub>s (subst [y \<mapsto> t']) e\<^sub>2', subst [y \<mapsto> t'] t\<^sub>2, vs''', constr_subst y t' con\<^sub>2)" by blast
   from App\<^sub>s E T1' T2' have "typecheck' (\<Gamma>(x \<mapsto> t')) vs (App\<^sub>s e1 e2) = 
-    (hsubst [y \<mapsto> t'] e', subst [y \<mapsto> t'] tt, vs', constr_subst y t' con)" by (auto simp add: Let_def)
+    (map_expr\<^sub>s (subst [y \<mapsto> t']) e', subst [y \<mapsto> t'] tt, vs', constr_subst y t' con)" by (auto simp add: Let_def)
   thus ?case by blast
 qed auto
 
 lemma typecheck_fails' [simp]: "map_option to_type \<circ> \<Gamma> \<turnstile>\<^sub>t e\<^sub>t : t \<Longrightarrow> finite vs \<Longrightarrow> 
   subst_vars \<Gamma> \<subseteq> vs \<Longrightarrow> valid_ty_subst \<Gamma> \<Longrightarrow> typecheck' \<Gamma> vs (erase e\<^sub>t) = (e', tt, vs', con) \<Longrightarrow> 
-  \<exists>s. partial_solidify vs (hsubst s e') = liquify e\<^sub>t \<and> 
+  \<exists>s. map_expr\<^sub>s (eliminate_vars vs) (map_expr\<^sub>s (subst s) e') = map_expr\<^sub>s to_unifiable e\<^sub>t \<and> 
   eliminate_vars vs (subst s tt) = to_unifiable t \<and> dom s = vs' - vs \<and> 
   subst_vars s = {} \<and> s unifies\<^sub>\<kappa> eliminate_vars_constr vs con \<and> valid_ty_subst s \<and> idempotent s"
 proof (induction "map_option to_type \<circ> \<Gamma>" e\<^sub>t t arbitrary: \<Gamma> vs e' tt vs' con rule: typing\<^sub>t.induct)
@@ -377,11 +351,11 @@ proof (induction "map_option to_type \<circ> \<Gamma>" e\<^sub>t t arbitrary: \<
   have Y: "(map_option to_type \<circ> \<Gamma>)(x \<mapsto> t\<^sub>1) = map_option to_type \<circ> (\<Gamma>(x \<mapsto> to_unifiable t\<^sub>1))" by simp
   from tc\<^sub>t_lam have Z: "valid_ty_subst (\<Gamma>(x \<mapsto> to_unifiable t\<^sub>1))" by simp
   from tc\<^sub>t_lam T have TC: "typecheck' (\<Gamma>(x \<mapsto> to_unifiable t\<^sub>1)) (insert ?v vs) (erase e) = 
-    (hsubst [?v \<mapsto> to_unifiable t\<^sub>1] e'', subst [?v \<mapsto> to_unifiable t\<^sub>1] t', vs'', 
+    (map_expr\<^sub>s (subst [?v \<mapsto> to_unifiable t\<^sub>1]) e'', subst [?v \<mapsto> to_unifiable t\<^sub>1] t', vs'', 
      constr_subst ?v (to_unifiable t\<^sub>1) con')" by simp
   from tc\<^sub>t_lam have "finite (insert ?v vs)" by simp
   with tc\<^sub>t_lam X Y Z TC obtain s where S: "
-    partial_solidify (insert ?v vs) (hsubst s (hsubst [?v \<mapsto> to_unifiable t\<^sub>1] e'')) = liquify e \<and> 
+    map_expr\<^sub>s (eliminate_vars (insert ?v vs)) (map_expr\<^sub>s (subst s) (map_expr\<^sub>s (subst [?v \<mapsto> to_unifiable t\<^sub>1]) e'')) = map_expr\<^sub>s to_unifiable e \<and> 
     eliminate_vars (insert ?v vs) (subst s (subst [?v \<mapsto> to_unifiable t\<^sub>1] t')) = to_unifiable t\<^sub>2 \<and>
     s unifies\<^sub>\<kappa> eliminate_vars_constr (insert ?v vs) (constr_subst ?v (to_unifiable t\<^sub>1) con') \<and> 
     dom s = vs'' - insert ?v vs \<and> subst_vars s = {} \<and> valid_ty_subst s \<and> idempotent s" by meson
@@ -389,17 +363,17 @@ proof (induction "map_option to_type \<circ> \<Gamma>" e\<^sub>t t arbitrary: \<
   moreover from tc\<^sub>t_lam have FV: "?v \<notin> vs" by simp
   ultimately have "?v \<notin> subst_vars (\<Gamma>(x \<mapsto> to_unifiable t\<^sub>1))" by blast
   with tc\<^sub>t_lam TC have VCS: "?v \<notin> constr_vars (constr_subst ?v (to_unifiable t\<^sub>1) con')" by simp
-  have "htvars (hsubst [?v \<mapsto> to_unifiable t\<^sub>1] e') \<subseteq> 
-    htvars e' - dom [?v \<mapsto> to_unifiable t\<^sub>1] \<union> subst_vars [?v \<mapsto> to_unifiable t\<^sub>1]" 
+  have "tyvars\<^sub>s (map_expr\<^sub>s (subst [?v \<mapsto> to_unifiable t\<^sub>1]) e') \<subseteq> 
+    tyvars\<^sub>s e' - dom [?v \<mapsto> to_unifiable t\<^sub>1] \<union> subst_vars [?v \<mapsto> to_unifiable t\<^sub>1]" 
       by (metis htvars_hsubst)
-  hence "htvars (hsubst [?v \<mapsto> to_unifiable t\<^sub>1] e') \<subseteq> htvars e' - {?v}" by simp
-  moreover have "htvars (hsubst s (hsubst [?v \<mapsto> to_unifiable t\<^sub>1] e')) \<subseteq> 
-    htvars (hsubst [?v \<mapsto> to_unifiable t\<^sub>1] e') - dom s \<union> subst_vars s" by simp
-  ultimately have "htvars (hsubst s (hsubst [?v \<mapsto> to_unifiable t\<^sub>1] e')) \<subseteq> 
-    htvars e' - {?v} - dom s \<union> subst_vars s" by blast
-  with S have "?v \<notin> htvars (hsubst (extend_subst ?v (to_unifiable t\<^sub>1) s) e')" by auto
-  with E S VCS have A: "partial_solidify vs (hsubst (extend_subst ?v (to_unifiable t\<^sub>1) s) e') = 
-    liquify (Lam\<^sub>s x t\<^sub>1 e)" by simp
+  hence "tyvars\<^sub>s (map_expr\<^sub>s (subst [?v \<mapsto> to_unifiable t\<^sub>1]) e') \<subseteq> tyvars\<^sub>s e' - {?v}" by simp
+  moreover have "tyvars\<^sub>s (map_expr\<^sub>s (subst s) (map_expr\<^sub>s (subst [?v \<mapsto> to_unifiable t\<^sub>1]) e')) \<subseteq> 
+    tyvars\<^sub>s (map_expr\<^sub>s (subst [?v \<mapsto> to_unifiable t\<^sub>1]) e') - dom s \<union> subst_vars s" by simp
+  ultimately have "tyvars\<^sub>s (map_expr\<^sub>s (subst s) (map_expr\<^sub>s (subst [?v \<mapsto> to_unifiable t\<^sub>1]) e')) \<subseteq> 
+    tyvars\<^sub>s e' - {?v} - dom s \<union> subst_vars s" by blast
+  with S have "?v \<notin> tyvars\<^sub>s (map_expr\<^sub>s (subst (extend_subst ?v (to_unifiable t\<^sub>1) s)) e')" by auto
+  with E S VCS have A: "map_expr\<^sub>s (eliminate_vars vs) (map_expr\<^sub>s (subst (extend_subst ?v (to_unifiable t\<^sub>1) s)) e') = 
+    map_expr\<^sub>s to_unifiable (Lam\<^sub>s x t\<^sub>1 e)" by simp
   from tc\<^sub>t_lam S have U: "?v \<notin> dom s" by auto
   with S have B: "idempotent (extend_subst ?v (to_unifiable t\<^sub>1) s)" by simp
   from S E FV have "s unifies\<^sub>\<kappa> constr_subst ?v (to_unifiable t\<^sub>1) (eliminate_vars_constr vs con)" 
@@ -439,7 +413,7 @@ next
     con = con\<^sub>1 @ con\<^sub>2 @ [(t\<^sub>1', Arrow\<^sub>\<tau> t\<^sub>2' (Var ?v))]" by (auto simp add: Let_def)
   from tc\<^sub>t_app have "subst_vars \<Gamma> \<subseteq> insert ?v vs" by auto
   with tc\<^sub>t_app TC1 obtain s\<^sub>1 where S1: "
-    partial_solidify (insert ?v vs) (hsubst s\<^sub>1 e\<^sub>1') = liquify e\<^sub>1 \<and> 
+    map_expr\<^sub>s (eliminate_vars (insert ?v vs)) (map_expr\<^sub>s (subst s\<^sub>1) e\<^sub>1') = map_expr\<^sub>s to_unifiable e\<^sub>1 \<and> 
     eliminate_vars (insert ?v vs) (subst s\<^sub>1 t\<^sub>1') = to_unifiable (Arrow t\<^sub>1 t\<^sub>2) \<and> 
     dom s\<^sub>1 = vs'' - insert ?v vs \<and> subst_vars s\<^sub>1 = {} \<and> 
     s\<^sub>1 unifies\<^sub>\<kappa> eliminate_vars_constr (insert ?v vs) con\<^sub>1 \<and> valid_ty_subst s\<^sub>1 \<and> idempotent s\<^sub>1" 
@@ -447,7 +421,7 @@ next
   from TC1 have V1: "insert ?v vs \<subseteq> vs''" by (metis vars_expand)
   from TC2 E have V2: "vs'' \<subseteq> vs'" by (metis vars_expand)
   with tc\<^sub>t_app V1 have Y: "subst_vars \<Gamma> \<subseteq> vs''" by auto
-  with tc\<^sub>t_app TC1 TC2 Y obtain s\<^sub>2 where S2: "partial_solidify vs'' (hsubst s\<^sub>2 e\<^sub>2') = liquify e\<^sub>2 \<and> 
+  with tc\<^sub>t_app TC1 TC2 Y obtain s\<^sub>2 where S2: "map_expr\<^sub>s (eliminate_vars vs'') (map_expr\<^sub>s (subst s\<^sub>2) e\<^sub>2') = map_expr\<^sub>s to_unifiable e\<^sub>2 \<and> 
     eliminate_vars vs'' (subst s\<^sub>2 t\<^sub>2') = to_unifiable t\<^sub>1 \<and> dom s\<^sub>2 = vs''' - vs'' \<and> subst_vars s\<^sub>2 = {} \<and> 
     s\<^sub>2 unifies\<^sub>\<kappa> eliminate_vars_constr vs'' con\<^sub>2 \<and> valid_ty_subst s\<^sub>2 \<and> idempotent s\<^sub>2" by fastforce
   from tc\<^sub>t_app have FV: "?v \<notin> vs" by simp
@@ -462,18 +436,26 @@ next
   with V1 V2 D1 have D3: "dom (combine_subst s\<^sub>1 s\<^sub>2) = vs' - insert ?v vs" by auto
   with FV V1 V2 have A: "dom ?s = vs' - vs" by auto
   from tc\<^sub>t_app have VG: "?v \<notin> subst_vars \<Gamma>" by auto 
-  with tc\<^sub>t_app TC1 have VE1: "?v \<notin> htvars e\<^sub>1'" by simp
-  from tc\<^sub>t_app TC1 TC2 V1 VG have VE2: "?v \<notin> htvars e\<^sub>2'" by simp
-  from tc\<^sub>t_app TC1 have "htvars e\<^sub>1' \<subseteq> vs'' - insert ?v vs" by simp
-  with D2 have HV: "dom s\<^sub>2 \<inter> htvars e\<^sub>1' = {}" by auto
-  from tc\<^sub>t_app E TC1 TC2 have HV2: "htvars e\<^sub>2' \<subseteq> vs' - vs''" by simp
-  have "htvars (hsubst s\<^sub>2 e\<^sub>2') \<subseteq> htvars e\<^sub>2' - dom s\<^sub>2 \<union> subst_vars s\<^sub>2" by simp
-  with D2 S2 HV2 have HVS2: "htvars (hsubst s\<^sub>2 e\<^sub>2') = {}" by auto
-  have "htvars (hsubst s\<^sub>1 e\<^sub>1') \<subseteq> htvars e\<^sub>1' - dom s\<^sub>1 \<union> subst_vars s\<^sub>1" by simp
-  with VE1 S1 have "?v \<notin> htvars (hsubst s\<^sub>1 e\<^sub>1')" by blast
-  with S1 S2 VE1 VE2 HV HVS2 have "partial_solidify vs (hsubst ?s e\<^sub>1') = liquify e\<^sub>1 \<and>
-    partial_solidify vs (hsubst ?s e\<^sub>2') = liquify e\<^sub>2" by simp
-  hence B: "partial_solidify vs (hsubst ?s (App\<^sub>s e\<^sub>1' e\<^sub>2')) = liquify (App\<^sub>s e\<^sub>1 e\<^sub>2)" by simp
+  with tc\<^sub>t_app TC1 have VE1: "?v \<notin> tyvars\<^sub>s e\<^sub>1'" by simp
+  from tc\<^sub>t_app TC1 TC2 V1 VG have VE2: "?v \<notin> tyvars\<^sub>s e\<^sub>2'" by simp
+  from tc\<^sub>t_app TC1 have "tyvars\<^sub>s e\<^sub>1' \<subseteq> vs'' - insert ?v vs" by simp
+  with D2 have HV: "dom s\<^sub>2 \<inter> tyvars\<^sub>s e\<^sub>1' = {}" by auto
+  from tc\<^sub>t_app E TC1 TC2 have HV2: "tyvars\<^sub>s e\<^sub>2' \<subseteq> vs' - vs''" by simp
+  have "tyvars\<^sub>s (map_expr\<^sub>s (subst s\<^sub>2) e\<^sub>2') \<subseteq> tyvars\<^sub>s e\<^sub>2' - dom s\<^sub>2 \<union> subst_vars s\<^sub>2" by simp
+  with D2 S2 HV2 have HVS2: "tyvars\<^sub>s (map_expr\<^sub>s (subst s\<^sub>2) e\<^sub>2') = {}" by auto
+  have "tyvars\<^sub>s (map_expr\<^sub>s (subst s\<^sub>1) e\<^sub>1') \<subseteq> tyvars\<^sub>s e\<^sub>1' - dom s\<^sub>1 \<union> subst_vars s\<^sub>1" by simp
+  with VE1 S1 have "?v \<notin> tyvars\<^sub>s (map_expr\<^sub>s (subst s\<^sub>1) e\<^sub>1')" by blast
+  with S1 HV have "map_expr\<^sub>s (eliminate_vars vs) (map_expr\<^sub>s (subst s\<^sub>1) (map_expr\<^sub>s (subst s\<^sub>2) e\<^sub>1')) = 
+    map_expr\<^sub>s to_unifiable e\<^sub>1" by simp
+  hence PS1: "map_expr\<^sub>s (eliminate_vars vs) (map_expr\<^sub>s (subst s\<^sub>1 \<circ> subst s\<^sub>2) e\<^sub>1') = map_expr\<^sub>s to_unifiable e\<^sub>1"
+    by (simp add: expr\<^sub>s.map_comp)
+  from S2 HVS2 have "map_expr\<^sub>s (eliminate_vars vs) (map_expr\<^sub>s (subst s\<^sub>1) (map_expr\<^sub>s (subst s\<^sub>2) e\<^sub>2')) = 
+    map_expr\<^sub>s to_unifiable e\<^sub>2" by simp
+  hence "map_expr\<^sub>s (eliminate_vars vs) (map_expr\<^sub>s (subst s\<^sub>1 \<circ> subst s\<^sub>2) e\<^sub>2') = map_expr\<^sub>s to_unifiable e\<^sub>2"
+    by (simp add: expr\<^sub>s.map_comp)
+  with VE1 VE2 PS1 have "map_expr\<^sub>s (eliminate_vars vs) (map_expr\<^sub>s (subst ?s) e\<^sub>1') = map_expr\<^sub>s to_unifiable e\<^sub>1 \<and>
+    map_expr\<^sub>s (eliminate_vars vs) (map_expr\<^sub>s (subst ?s) e\<^sub>2') = map_expr\<^sub>s to_unifiable e\<^sub>2" by simp
+  hence B: "map_expr\<^sub>s (eliminate_vars vs) (map_expr\<^sub>s (subst ?s) (App\<^sub>s e\<^sub>1' e\<^sub>2')) = map_expr\<^sub>s to_unifiable (App\<^sub>s e\<^sub>1 e\<^sub>2)" by simp
   have C: "eliminate_vars vs (subst ?s (Var ?v)) = to_unifiable t\<^sub>2" by simp
   from S1 S2 DSS D3 have D: "subst_vars ?s = {}" by auto
   from S1 S2 have VCS: "?v \<notin> subst_vars s\<^sub>1 \<and> ?v \<notin> subst_vars s\<^sub>2" by auto
@@ -535,7 +517,7 @@ proof
   then obtain e\<^sub>t t where Y: "(map_option to_type \<circ> Map.empty \<turnstile>\<^sub>t e\<^sub>t : t) \<and> e = erase e\<^sub>t" by fastforce
   have Z: "subst_vars Map.empty \<subseteq> {}" by simp
   have "valid_ty_subst Map.empty \<and> finite {}" by simp
-  with X Y Z have "\<exists>s. partial_solidify {} (hsubst s e') = liquify e\<^sub>t \<and> 
+  with X Y Z have "\<exists>s. map_expr\<^sub>s (eliminate_vars {}) (map_expr\<^sub>s (subst s) e') = map_expr\<^sub>s to_unifiable e\<^sub>t \<and> 
     eliminate_vars {} (subst s tt) = to_unifiable t \<and> dom s = vs' - {} \<and> subst_vars s = {} \<and> 
     s unifies\<^sub>\<kappa> eliminate_vars_constr {} con \<and> valid_ty_subst s \<and> idempotent s" 
     using typecheck_fails' by blast
