Compiler.thy
@@ -115,10 +115,12 @@ definition alg_compile :: "unit expr\<^sub>s \<rightharpoonup> mach list \<times
       | Some s \<Rightarrow> 
           Some (alg_compile3 (alg_compile2 0 (alg_compile1 [] e []) []), to_type (subst s t)))"
 
-lemma [simp]: "encode (convert' \<Phi> (solidify (hsubst sub e))) = encode (convert' \<Phi> (solidify e))"
+lemma [simp]: "encode (convert' \<Phi> (map_expr\<^sub>s to_type (map_expr\<^sub>s (subst sub) e))) = 
+    encode (convert' \<Phi> (map_expr\<^sub>s to_type e))"
   by (induction e arbitrary: \<Phi>) simp_all
 
-lemma [simp]: "encode \<circ> convert \<circ> solidify \<circ> hsubst sub = encode \<circ> convert \<circ> solidify"
+lemma [simp]: "encode \<circ> convert \<circ> map_expr\<^sub>s to_type \<circ> map_expr\<^sub>s (subst sub) = 
+    encode \<circ> convert \<circ> map_expr\<^sub>s to_type"
   by (auto simp add: convert_def)
 
 lemma [simp]: "typecheck' \<Gamma> vs e = (e', t, vs', con) \<Longrightarrow> quick_convert vs e = (e', vs')"
@@ -126,11 +128,11 @@ lemma [simp]: "typecheck' \<Gamma> vs e = (e', t, vs', con) \<Longrightarrow> qu
      (simp_all add: Let_def split: option.splits prod.splits)
 
 lemma [simp]: "quick_convert vs e = (e', vs') \<Longrightarrow> 
-    alg_compile1 \<Phi> e acc = encode (convert' \<Phi> (solidify e')) @ acc"
+    alg_compile1 \<Phi> e acc = encode (convert' \<Phi> (map_expr\<^sub>s to_type e')) @ acc"
   by (induction e arbitrary: \<Phi> acc vs e' vs') (auto simp add: Let_def split: prod.splits)
 
 lemma [simp]: "typecheck' \<Gamma> vs e = (e', t, vs', con) \<Longrightarrow> 
-  alg_compile1 \<Phi> e acc = encode (convert' \<Phi> (solidify e')) @ acc"
+  alg_compile1 \<Phi> e acc = encode (convert' \<Phi> (map_expr\<^sub>s to_type e')) @ acc"
 proof -
   assume "typecheck' \<Gamma> vs e = (e', t, vs', con)"
   hence "quick_convert vs e = (e', vs')" by simp
